pancake/proofs/pan_to_wordProofScript.sml
@@ -3,10 +3,16 @@
 *)
 
 open preamble pan_to_wordTheory
-     pan_to_crepProofTheory crep_to_loopProofTheory
-     loop_to_wordProofTheory
+     pan_simpProofTheory pan_to_crepProofTheory
+     crep_to_loopProofTheory loop_to_wordProofTheory
 
 val _ = new_theory "pan_to_wordProof";
+
+
+Definition pan_simp_st_def:
+  pan_simp_st (s:('a,'ffi) panSem$state) (pan_code:(mlstring # (mlstring # shape) list # α prog) list) =
+    s with code := alist_to_fmap (pan_simp$compile_prog pan_code)
+End
 
 
 Definition crep_state_def:
@@ -41,6 +47,48 @@ Definition loop_state_def:
      ffi      := s.ffi|>
 End
 
+
+Definition consistent_labels_def:
+  consistent_labels (mem:'a word -> 'a word_lab)
+                    (pan_code:(mlstring # (mlstring # shape) list # α prog) list) <=>
+  ∀ad f.
+   mem ad = Label f ⇒
+   ∃n m. FLOOKUP (make_funcs (compile_prog (pan_simp$compile_prog pan_code))) f = SOME (n,m)
+End
+
+
+Theorem FDOM_get_eids_pan_simp_compile_eq:
+  !prog. FDOM ((get_eids prog): mlstring |-> α word) =
+  FDOM ((get_eids (pan_simp$compile_prog prog)):mlstring |-> α word)
+Proof
+  rw [] >>
+  fs [pan_to_crepTheory.get_eids_def] >>
+  qmatch_goalsub_abbrev_tac ‘BIGUNION es’ >>
+  qmatch_goalsub_abbrev_tac ‘_ = set (MAP FST (MAP2 (λx y. (x,y))
+    (SET_TO_LIST (BIGUNION ces)) _ ))’ >>
+  qsuff_tac ‘es = ces’
+  >- fs [] >>
+  fs [Abbr ‘es’, Abbr ‘ces’, pan_simpTheory.compile_prog_def] >>
+  fs [MAP_MAP_o] >>
+  fs [pan_simpProofTheory.map_snd_f_eq] >>
+  fs [GSYM LIST_TO_SET_MAP] >>
+  qsuff_tac ‘MAP exp_ids (MAP compile (MAP (SND ∘ SND) prog)) =
+             MAP exp_ids (MAP (SND ∘ SND) prog)’
+  >- fs [] >>
+  fs [MAP_EQ_EVERY2, LIST_REL_EL_EQN] >>
+  rw [] >>
+  ‘n < LENGTH  (MAP (SND ∘ SND) prog)’ by fs [] >>
+  drule (INST_TYPE [``:'a``|->``:'c``,
+                    ``:'b``|->``:'c``] EL_MAP) >>
+  disch_then (qspec_then ‘pan_simp$compile’ mp_tac) >>
+  fs [] >>
+  strip_tac >>
+  fs [exp_ids_compile_eq]
+QED
+
+
+
+(*
 Theorem first_compile_prog_all_distinct:
   ALL_DISTINCT (MAP FST pan_code) ==>
   ALL_DISTINCT
@@ -52,7 +100,7 @@ Theorem first_compile_prog_all_distinct:
 Proof
   rw [] >>
   qmatch_goalsub_abbrev_tac ‘MAP _ cs’ >>
-  ‘MAP FST cs = MAP FST cs’
+  ‘MAP FST cs = MAP FST pan_code’ >>
 
 
   fs [pan_to_crepTheory.compile_prog_def] >>
@@ -108,12 +156,13 @@ Proof
    cheat) >>
   cheat
 QED
-
+*)
 
 Theorem state_rel_imp_semantics:
   t.memory = mk_mem
              (mk_ctxt FEMPTY (make_funcs (compile_prog pan_code)) 0
               (get_eids (compile_prog pan_code))) s.memory /\
+  consistent_labels s.memory pan_code /\
   t.mdomain = s.memaddrs ∧
   t.be = s.be ∧
   t.ffi = s.ffi ∧
@@ -123,50 +172,146 @@ Theorem state_rel_imp_semantics:
   t.code = fromAList (pan_to_word$compile_prog pan_code) ∧
   s.locals = FEMPTY ∧ size_of_eids pan_code < dimword (:α) ∧
   FDOM s.eshapes = FDOM ((get_eids pan_code):mlstring |-> 'a word) ∧
-  (∀ad f.
-   s.memory ad = Label f ⇒
-   ∃n m. FLOOKUP (make_funcs (compile_prog pan_code)) f = SOME (n,m)) /\
-  FLOOKUP (make_funcs (compile_prog pan_code)) start = SOME (lc,0) /\
+  FLOOKUP (make_funcs (compile_prog (pan_simp$compile_prog pan_code))) start = SOME (lc,0) /\
   lookup 0 t.locals = SOME (Loc 1 0) /\
   semantics s start <> Fail ==>
   semantics (t:('a,'b, 'ffi) wordSem$state) lc =
   semantics (s:('a,'ffi) panSem$state) start
 Proof
   rw [] >>
-  ‘state_rel s (crep_state s pan_code)’ by (
-    fs [pan_to_crepProofTheory.state_rel_def, crep_state_def]) >>
-  drule (GEN_ALL pan_to_crepProofTheory.state_rel_imp_semantics) >>
-  disch_then (qspecl_then [‘start’, ‘prog’ , ‘pan_code’] mp_tac) >>
+  (* pan-simp pass *)
+  ‘state_rel s (pan_simp_st s pan_code) (pan_simp_st s pan_code).code’ by (
+    fs [pan_simpProofTheory.state_rel_def, pan_simp_st_def] >>
+    conj_tac >> rw []
+    >- (
+     fs [pan_simpTheory.compile_prog_def] >>
+     fs [ALOOKUP_FAILS] >>
+     rw [] >>
+     fs [MEM_MAP] >>
+     rw [] >>
+     cases_on ‘y’ >>
+     cases_on ‘r’ >> fs [] >>
+     CCONTR_TAC >> fs [] >>
+     rveq >> fs [] >> metis_tac []) >>
+    fs [pan_simpTheory.compile_prog_def] >>
+    fs [ALOOKUP_EXISTS_IFF] >>
+    match_mp_tac ALOOKUP_ALL_DISTINCT_MEM >>
+    conj_tac
+    >- (
+     fs [MAP_MAP_o] >>
+     qmatch_goalsub_abbrev_tac ‘MAP ff _’ >>
+     ‘MAP ff pan_code = MAP FST pan_code’ by (
+       fs [Abbr ‘ff’, MAP_EQ_f] >>
+       rw [] >>
+       cases_on ‘e’ >> fs [] >>
+       cases_on ‘r’ >> fs []) >>
+     fs []) >>
+    fs [MEM_MAP] >>
+    qexists_tac ‘(f,vshs,prog')’ >>
+    fs [] >>
+    drule ALOOKUP_MEM >> fs []) >>
+  drule pan_simpProofTheory.state_rel_imp_semantics >>
+  disch_then (qspecl_then [‘pan_code’, ‘start’, ‘prog’] mp_tac) >>
   fs [] >>
-  impl_tac
-  >- fs [crep_state_def] >>
+  impl_tac >- fs [pan_simp_st_def] >>
   strip_tac >>
   pop_assum (assume_tac o GSYM) >>
   fs [] >>
-  ‘(crep_state s pan_code).memaddrs =
-   (loop_state (crep_state s pan_code) (pan_to_crep$compile_prog pan_code) t.clock).mdomain’ by
-    fs [crep_state_def, loop_state_def] >>
-  drule (GEN_ALL crep_to_loopProofTheory.state_rel_imp_semantics) >>
-  disch_then (qspecl_then [‘start’, ‘comp_func (make_funcs pan_code) (get_eids pan_code) [] prog’,
-                           ‘lc’, ‘compile_prog pan_code’] mp_tac) >>
+  qmatch_goalsub_abbrev_tac ‘semantics pst start’ >>
+ (* pan_to_crep pass *)
+  ‘state_rel pst (crep_state pst (pan_simp$compile_prog pan_code))’ by (
+    fs [pan_to_crepProofTheory.state_rel_def, crep_state_def]) >>
+  drule pan_to_crepProofTheory.state_rel_imp_semantics >>
+  disch_then (qspecl_then [‘pan_simp$compile_prog pan_code’,
+                           ‘start’, ‘pan_simp$compile prog’] mp_tac) >>
+  fs [] >>
   impl_tac
   >- (
-   fs [crep_state_def, loop_state_def] >>
+   fs [Abbr ‘pst’, pan_simp_st_def, crep_state_def] >>
+   conj_tac
+   >- (
+    match_mp_tac pan_simpProofTheory.first_compile_prog_all_distinct >>
+    fs []) >>
+   fs [size_of_eids_compile_eq] >>
+   fs [Once FDOM_get_eids_pan_simp_compile_eq] >>
+   fs [pan_simpTheory.compile_prog_def] >>
+   match_mp_tac ALOOKUP_ALL_DISTINCT_MEM >>
+   conj_tac
+   >- (
+    fs [MAP_MAP_o] >>
+    qmatch_goalsub_abbrev_tac ‘MAP ff _’ >>
+    ‘MAP ff pan_code = MAP FST pan_code’ by (
+      fs [Abbr ‘ff’, MAP_EQ_f] >>
+      rw [] >>
+      cases_on ‘e’ >> fs [] >>
+      cases_on ‘r’ >> fs []) >>
+    fs []) >>
+   fs [MEM_MAP] >>
+   qexists_tac ‘(start,[],prog)’ >>
+   fs [] >>
+   drule ALOOKUP_MEM >> fs []) >>
+  strip_tac >>
+  pop_assum (assume_tac o GSYM) >>
+  fs [] >>
+  qmatch_goalsub_abbrev_tac ‘semantics cst start’ >>
+
+
+
+  (* crep_to_loop pass *)
+  ‘cst.memaddrs =
+   (loop_state cst (pan_to_crep$compile_prog (pan_simp$compile_prog pan_code)) t.clock).mdomain’ by
+    fs [Abbr ‘cst’, Abbr ‘pst’, crep_state_def, loop_state_def] >>
+  drule crep_to_loopProofTheory.state_rel_imp_semantics >>
+  disch_then (qspecl_then [‘compile_prog (pan_simp$compile_prog pan_code)’,
+                           ‘start’, ‘comp_func (make_funcs (pan_simp$compile_prog pan_code))
+                                     (get_eids (pan_simp$compile_prog pan_code)) [] (compile prog)’,
+                           ‘lc’] mp_tac) >>
+  impl_tac
+  >- (
+   fs [Abbr ‘pst’, Abbr ‘cst’, pan_simp_st_def, crep_state_def, loop_state_def] >>
    conj_tac
    >- (
     fs [crep_to_loopTheory.mk_ctxt_def, mk_mem_def, mem_rel_def] >>
     rw [] >> res_tac >> rfs []) >>
    conj_tac
-   >- fs [get_eids_equivs] >>
+   >- cheat (* fs [get_eids_equivs] *) >>
    conj_tac >- fs [crep_to_loopProofTheory.globals_rel_def] >>
-   conj_tac >- metis_tac [first_compile_prog_all_distinct] >>
-   metis_tac [alookup_compile_prog_code]) >>
+   conj_tac
+   >-  (
+    match_mp_tac first_compile_prog_all_distinct >>
+    match_mp_tac pan_simpProofTheory.first_compile_prog_all_distinct >>
+    fs []) >>
+   match_mp_tac alookup_compile_prog_code >>
+   conj_tac
+   >- (
+    match_mp_tac pan_simpProofTheory.first_compile_prog_all_distinct >>
+    fs []) >>
+   fs [pan_simpTheory.compile_prog_def] >>
+   match_mp_tac ALOOKUP_ALL_DISTINCT_MEM >>
+   conj_tac
+   >- (
+    fs [MAP_MAP_o] >>
+    qmatch_goalsub_abbrev_tac ‘MAP ff _’ >>
+    ‘MAP ff pan_code = MAP FST pan_code’ by (
+      fs [Abbr ‘ff’, MAP_EQ_f] >>
+      rw [] >>
+      cases_on ‘e’ >> fs [] >>
+      cases_on ‘r’ >> fs []) >>
+    fs []) >>
+   fs [MEM_MAP] >>
+   qexists_tac ‘(start,[], prog)’ >>
+   fs [] >>
+   drule ALOOKUP_MEM >> fs []) >>
   strip_tac >>
   pop_assum (assume_tac o GSYM) >>
   fs [] >>
   pop_assum kall_tac >>
+  qmatch_goalsub_abbrev_tac ‘_ = semantics lst _’ >>
+  (* loop_to_word pass *)
+
+
   match_mp_tac (GEN_ALL fstate_rel_imp_semantics) >>
-  MAP_EVERY qexists_tac [‘ARB’, ‘compile_prog (compile_prog pan_code)’] >>
+  MAP_EVERY qexists_tac [‘ARB’, ‘compile_prog (compile_prog (compile_prog pan_code))’] >>
   fs [] >>
   conj_tac
   >- (
@@ -174,21 +319,37 @@ Proof
    conj_tac
    >- (
     fs [loop_removeProofTheory.state_rel_def] >>
-    qexists_tac ‘fromAList (comp_prog (compile_prog (compile_prog pan_code)))’ >>
+    qexists_tac ‘fromAList (comp_prog (compile_prog (compile_prog (compile_prog pan_code))))’ >>
     fs [] >>
     rpt gen_tac >>
     strip_tac >>
-    fs [loop_state_def, crep_state_def] >>
+    fs [loop_state_def, crep_state_def, pan_simp_st_def] >>
     cheat) >>
-   fs [loop_to_wordProofTheory.state_rel_def] >>
-   fs [loop_state_def, crep_state_def] >>
+   fs [Abbr ‘lst’, loop_to_wordProofTheory.state_rel_def] >>
+   fs [loop_state_def, crep_state_def, pan_simp_st_def] >>
    fs [globals_rel_def] >>
    fs [] >>
-   fs [loop_to_wordProofTheory.code_rel_def] >>
-   rpt gen_tac >>
-   strip_tac >>
    conj_tac
    >- (
+    conj_tac
+    >- (
+     fs []
+
+     )
+
+    )
+
+
+
+
+
+   fs [loop_to_wordProofTheory.code_rel_def] >>
+   conj_tac
+   >- (
+    rpt gen_tac >>
+    strip_tac >>
+    conj_tac
+    >- (
     fs [pan_to_wordTheory.compile_prog_def,
         loop_to_wordTheory.compile_def] >>
     fs [loop_to_wordTheory.compile_prog_def] >>
